theories/Relational/RelationalExcFull.v
@@ -6,215 +6,259 @@ From Mon.SRelation Require Import SRelation_Definitions SMorphisms.
 From Mon.sprop Require Import SPropBase SPropMonadicStructures MonadExamples SpecificationMonads.
 From Relational Require Import OrderEnrichedCategory OrderEnrichedRelativeMonadExamples Rel GenericRulesComplex.
 
-
 Set Universe Polymorphism.
 
-Definition M01 := Exn unit.
-Definition M02 := Identity.
-Definition W01 := ExnSpec unit.
-Definition W02 := MonoContSProp.
+Module ExcId.
+  Definition M01 := Exn unit.
+  Definition M02 := Identity.
+  Definition W01 := ExnSpec unit.
+  Definition W02 := MonoContSProp.
 
-Definition M1 := monad_to_relmon M01.
-Definition M2 := monad_to_relmon M02.
-Definition W1 := ordmonad_to_relmon W01.
-Definition W2 := ordmonad_to_relmon W02.
+  Definition M1 := monad_to_relmon M01.
+  Definition M2 := monad_to_relmon M02.
+  Definition W1 := ordmonad_to_relmon W01.
+  Definition W2 := ordmonad_to_relmon W02.
 
-Import SPropNotations.
-Import RelNotations.
+  Import SPropNotations.
+  Import RelNotations.
 
-Program Definition Wrel0 (A : TypeCatSq) : OrdCat :=
-  dpair _ (MonoContSProp (option (nfst A) × (nsnd A))) ⦑@omon_rel _ _⦒.
-Next Obligation. apply: MonoCont_order_preorder. Qed.
-
-Notation " X --> Y " := (X -> dfst Y) (at level 99).
-
-Program Definition retWrel0 (A : TypeCatSq) : OrdCat⦅ Jprod A; Wrel0 A⦆ :=
-  let f : (typeCat_prod A --> Wrel0 A) :=
-      fun a12 => ⦑fun p => p ⟨Some (nfst a12), nsnd a12⟩⦒
-  in to_discr f.
-Next Obligation. cbv ; intuition. Qed.
-
-Program Definition actWrel0 A1 A2 B1 B2 :
-  OrdCat ⦅ discr A1; W1 B1 ⦆ ->
-  OrdCat ⦅ discr A2; W2 B2 ⦆ ->
-  OrdCat ⦅ Jprod ⟨ A1, A2 ⟩; Wrel0 ⟨ B1, B2 ⟩ ⦆ ->
-  OrdCat ⦅ Wrel0 ⟨ A1, A2 ⟩; Wrel0 ⟨ B1, B2 ⟩ ⦆ :=
-  fun wf1 wf2 wfrel =>
-    ⦑fun wm =>
-       ⦑fun p =>
-          let k a12 :=
-              match nfst a12 with
-              | Some a1 => (wfrel∙1 ⟨a1, nsnd a12⟩)∙1 p
-              | None => (wf2∙1 (nsnd a12))∙1 (fun b2 => p ⟨None, b2⟩)
-              end
-          in wm∙1 k⦒⦒.
-Next Obligation.
-  move=> ? ? H; apply: wm∙2 => -[[?|] ?] /=;
-    by [apply: (wfrel∙1 _)∙2| apply: (wf2∙1 _)∙2].
-Qed.
-Next Obligation. cbv;intuition. Qed.
-
-Program Definition Wrc : rsm_components W1 W2 :=
-  mkRSMComponents _ _ Wrel0 retWrel0 actWrel0 _ _ _ _.
-Next Obligation.
-  move=> ? ? H ? ? H1 ? ? H2 w ? /=.
-  apply: w∙2=> -[[?|] ?] /=; [apply: H2| apply: H1].
-Qed.
-Next Obligation.
-  apply Ssig_eq=> /=.
-  extensionality wm. apply Ssig_eq. extensionality p=> /=.
-  f_equal. extensionality a; move: a => [[?|] ?] //=.
-Qed.
-
-Definition Wrel : RelationalSpecMonad := mkRSM W1 W2 Wrc.
+  Program Definition Wrel0 (A : TypeCatSq) : OrdCat :=
+    dpair _ (MonoContSProp (option (nfst A) × (nsnd A))) ⦑@omon_rel _ _⦒.
+  Next Obligation. apply: MonoCont_order_preorder. Qed.
 
 
+  Program Definition retWrel0 (A : TypeCatSq) : OrdCat⦅ Jprod A; Wrel0 A⦆ :=
+    let f : (typeCat_prod A --> Wrel0 A) :=
+        fun a12 => ⦑fun p => p ⟨Some (nfst a12), nsnd a12⟩⦒
+    in to_discr f.
+  Next Obligation. cbv ; intuition. Qed.
 
-Definition θ01_helper {A} (m : M01 A) (p: A -> SProp) (pexc: unit -> SProp)
-  : SProp :=
-  match m with
-  | retFree _ a => p a
-  | opr _ => pexc tt
-  end.
+  Program Definition actWrel0 A1 A2 B1 B2 :
+    OrdCat ⦅ discr A1; W1 B1 ⦆ ->
+    OrdCat ⦅ discr A2; W2 B2 ⦆ ->
+    OrdCat ⦅ Jprod ⟨ A1, A2 ⟩; Wrel0 ⟨ B1, B2 ⟩ ⦆ ->
+    OrdCat ⦅ Wrel0 ⟨ A1, A2 ⟩; Wrel0 ⟨ B1, B2 ⟩ ⦆ :=
+    fun wf1 wf2 wfrel =>
+      ⦑fun wm =>
+        ⦑fun p =>
+            let k a12 :=
+                match nfst a12 with
+                | Some a1 => (wfrel∙1 ⟨a1, nsnd a12⟩)∙1 p
+                | None => (wf2∙1 (nsnd a12))∙1 (fun b2 => p ⟨None, b2⟩)
+                end
+            in wm∙1 k⦒⦒.
+  Next Obligation.
+    move=> ? ? H; apply: wm∙2 => -[[?|] ?] /=;
+      by [apply: (wfrel∙1 _)∙2| apply: (wf2∙1 _)∙2].
+  Qed.
+  Next Obligation. cbv;intuition. Qed.
 
-Program Definition θ01 : MonadMorphism M01 W01 :=
-  @mkMorphism M01 W01 (fun A m => ⦑θ01_helper m⦒(* ⦑fun p pexc => *)
-                               (*    match m with *)
-                               (*    | retFree _ a1 => p a1 *)
-                               (*    | opr _ => pexc tt *)
-                               (*    end⦒ *)) _ _.
-Next Obligation.
-  move=> ? ? H ? ? Hexc; move: m=> [?|? ?]; [apply: H| apply: Hexc].
-Qed.
-Next Obligation.
-  apply Ssig_eq. extensionality p. extensionality pexc=> /=.
-  move: m =>[?|? ?] //=.
-Qed.
+  Program Definition Wrc : rsm_components W1 W2 :=
+    mkRSMComponents _ _ Wrel0 retWrel0 actWrel0 _ _ _ _.
+  Next Obligation.
+    move=> ? ? H ? ? H1 ? ? H2 w ? /=.
+    apply: w∙2=> -[[?|] ?] /=; [apply: H2| apply: H1].
+  Qed.
+  Next Obligation.
+    apply Ssig_eq=> /=.
+    extensionality wm. apply Ssig_eq. extensionality p=> /=.
+    f_equal. extensionality a; move: a => [[?|] ?] //=.
+  Qed.
 
-
-Program Definition θ02 : MonadMorphism M02 W02 :=
-  @mkMorphism M02 W02 (fun A m => ret m) _ _.
-
-Definition θ1 := mmorph_to_rmmorph θ01.
-Definition θ2 := mmorph_to_rmmorph θ02.
-
-Program Definition θrc : reo_components M1 M2 Wrc θ1 θ2:=
-  mkREOComponents M1 M2 Wrc θ1 θ2
-                  (fun A =>
-                     let f : M1 (nfst A) × M2 (nsnd A) --> Wrc A :=
-                         fun m12 => ⦑fun p => match nfst m12 with
-                                        | retFree _ a1 => p ⟨Some a1, nsnd m12⟩
-                                        | opr _ => p ⟨None, nsnd m12⟩
-                                        end⦒
-                     in to_discr f) _ _.
-Next Obligation. move: m12 => [[?|? ?] ?] ? ?; apply. Qed.
-Next Obligation.
-  apply Ssig_eq; extensionality m12; move: m12 => [[?|??]?] //=.
-Qed.
-
-Definition θ : relationalEffectObservation M1 M2 Wrel :=
-  mkREO _ _ Wrel θ1 θ2 θrc.
+  Definition Wrel : RelationalSpecMonad := mkRSM W1 W2 Wrc.
 
 
-(** FIXME: Copy-paste from GenericRulesComplex *)
-Let valid := valid M01 M02 Wrel θ.
-Let mk_progSpec := mk_progSpec M01 M02 Wrel.
 
-Notation " Γ ⊫ c1 ≈ c2 [{ w1 , w2 , w }] " :=
-  (valid Γ _ _ (mk_progSpec Γ _ _ c1 w1 c2 w2 w))
-      (at level 85).
+  Definition θ01_helper {A} (m : M01 A) (p: A -> SProp) (pexc: unit -> SProp)
+    : SProp :=
+    match m with
+    | retFree _ a => p a
+    | opr _ => pexc tt
+    end.
 
-Ltac destruct_valid :=
-  unshelve econstructor; [split=> /= γ|move=> /= γl γr γw]; constructor.
-(** FIXME: Copy-paste from GenericRulesComplex *)
-
-Program Definition raise_spec {Γ} : Γ --> W1 False :=
-  fun=>⦑fun p pexc => pexc tt⦒.
-Next Obligation. cbv ; intuition. Qed.
-
-Program Definition rel_raise_spec {Γ A2} (a2: πr Γ -> A2) : ⟬Γ⟭ --> Wrc ⟨False, A2⟩ :=
-  fun γ => ⦑fun p => p ⟨None, a2 (πr γ)⟩⦒.
-Next Obligation. cbv ; intuition. Qed.
-
-Lemma ValidRaise Γ A2 (a2: _ -> A2) :
-  Γ ⊫ fun=> raise tt ≈ ret \o a2 [{raise_spec, retW \o a2, rel_raise_spec a2}].
-Proof. destruct_valid; cbv ; intuition. Qed.
+  Program Definition θ01 : MonadMorphism M01 W01 :=
+    @mkMorphism M01 W01 (fun A m => ⦑θ01_helper m⦒(* ⦑fun p pexc => *)
+                                (*    match m with *)
+                                (*    | retFree _ a1 => p a1 *)
+                                (*    | opr _ => pexc tt *)
+                                (*    end⦒ *)) _ _.
+  Next Obligation.
+    move=> ? ? H ? ? Hexc; move: m=> [?|? ?]; [apply: H| apply: Hexc].
+  Qed.
+  Next Obligation.
+    apply Ssig_eq. extensionality p. extensionality pexc=> /=.
+    move: m =>[?|? ?] //=.
+  Qed.
 
 
-Definition catchStr {Γ E A} (m : Γ -> Exn E A) (merr : Γ × E -> Exn E A)
-  : Γ -> Exn E A := fun γ => catch (m γ) (fun e => merr ⟨γ,e⟩).
+  Program Definition θ02 : MonadMorphism M02 W02 :=
+    @mkMorphism M02 W02 (fun A m => ret m) _ _.
 
-(* Program Definition catch_spec {A1} (w:W1 A1) (werr : unit -> W1 A1) : W1 A1 := *)
-(*   ⦑fun p pexc => w∙1 p (fun u => (werr u)∙1 p pexc)⦒. *)
-(* Next Obligation. *)
-(*   cbv ; intuition. *)
-(*   move: H1; apply: w∙2=> // ?; apply (werr _)∙2 => //. *)
-(* Qed. *)
+  Definition θ1 := mmorph_to_rmmorph θ01.
+  Definition θ2 := mmorph_to_rmmorph θ02.
 
-Program Definition catch_spec_str {Γ A1} (w:Γ --> W1 A1)
-        (werr : Γ × unit --> W1 A1) : Γ --> W1 A1 :=
-  fun γ => ⦑fun p pexc => (w γ)∙1 p (fun u => (werr ⟨γ,u⟩)∙1 p pexc)⦒.
-Next Obligation.
-  cbv ; intuition.
-  move: H1; apply: (w _)∙2=> // ?; apply (werr _)∙2 => //.
-Qed.
+  Program Definition θrc : reo_components M1 M2 Wrc θ1 θ2:=
+    mkREOComponents M1 M2 Wrc θ1 θ2
+                    (fun A =>
+                      let f : M1 (nfst A) × M2 (nsnd A) --> Wrc A :=
+                          fun m12 => ⦑fun p => match nfst m12 with
+                                          | retFree _ a1 => p ⟨Some a1, nsnd m12⟩
+                                          | opr _ => p ⟨None, nsnd m12⟩
+                                          end⦒
+                      in to_discr f) _ _.
+  Next Obligation. move: m12 => [[?|? ?] ?] ? ?; apply. Qed.
+  Next Obligation.
+    apply Ssig_eq; extensionality m12; move: m12 => [[?|??]?] //=.
+  Qed.
 
-(* Program Definition rel_catch_spec {A1 A2} (wmrel : Wrel A1 A2) *)
-(*            (wmerr : unit -> W1 A1) (* (wmerr_rel : unit -> Wrel A1 A2) *) *)
-(*   : Wrel A1 A2 := *)
-(*   ⦑fun p => wmrel∙1 (fun ae12 => match nfst ae12 with *)
-(*                            | Some a1 => p ⟨Some a1, nsnd ae12⟩ *)
-(*                            | None => (wmerr tt)∙1 (fun a1 => p ⟨Some a1, nsnd ae12⟩) *)
-(*                                               (fun u => p ⟨None, nsnd ae12⟩) *)
-(*                            end)⦒. *)
-
-(* Next Obligation. *)
-(*   cbv. move=> p1 p2 Hp ; apply: (wmrel)∙2=> [[[?|] ?]] ; first by apply: Hp. *)
-(*   apply: (wmerr _)∙2=> ?; apply: Hp. *)
-(* Qed. *)
-
-Program Definition rel_catch_spec_str
-        {Γ A1 A2} (wmrel : ⟬Γ⟭ --> Wrc ⟨A1, A2⟩)
-        (wmerr_rel : ⟬extends Γ unit A2⟭ --> Wrc ⟨A1, A2⟩)
-        (* (wmerr : πl Γ × unit --> W1 A1) *)
-  : ⟬Γ⟭ --> Wrc ⟨A1, A2⟩ :=
-  fun γ =>
-    ⦑fun p =>
-       let k ae12 :=
-           match nfst ae12 with
-           | Some a1 => p ⟨Some a1, nsnd ae12⟩
-           | None =>
-             (wmerr_rel (extend_point γ tt (nsnd ae12)))∙1 p
-             (* (wmerr ⟨πl γ, tt⟩)∙1 (fun a1 => p ⟨Some a1, nsnd ae12⟩) *)
-             (*                          (fun u => p ⟨None, nsnd ae12⟩) *)
-           end
-       in
-       (wmrel γ)∙1 k⦒.
-Next Obligation.
-  cbv. move=> p1 p2 Hp ; apply: (wmrel _)∙2=> [[[?|] ?]] ; first by apply: Hp.
-  apply: (wmerr_rel _)∙2=> ?; apply: Hp.
-Qed.
+  Definition θ : relationalEffectObservation M1 M2 Wrel :=
+    mkREO _ _ Wrel θ1 θ2 θrc.
 
 
-Lemma ValidCatch Γ A1 A2 (m1 : _ -> M1 A1) wm1
-      (m2: _ -> M2 A2) wm2 wmrel merr wmerr wmerr_rel:
-  Γ ⊫ m1 ≈ m2 [{wm1, wm2, wmrel}] ->
-  extends Γ unit A2 ⊫ merr ≈ ret \o nsnd [{wmerr, retW \o nsnd, wmerr_rel}] ->
-  Γ ⊫ catchStr m1 merr ≈ m2
-    [{catch_spec_str wm1 wmerr, wm2, rel_catch_spec_str wmrel wmerr_rel}].
-Proof.
-  move=> [[/= H1 H2] H] [[/= He1 He2] He]; destruct_valid.
-  - move=> p pexc /=.
-    move: (unbox (H1 γ)); unfold θ01_helper, catchStr.
-    move: (m1 γ) => [?|[[]]?] /=; first apply.
-    set pexc' := (pexc in SProp_op_order _ (_ _ pexc)).
-    move=> /(fun f => f p pexc') Htt.
-    estransitivity; [apply: (unbox (He1 ⟨γ, tt⟩)) | exact Htt].
-  - apply: (unbox (H2 _)).
-  - move=> p /=.
-    move: (unbox (H γl γr γw)); unfold θ01_helper, catchStr.
-    move: (m1 γl) => [?|[[]]?] /=; first apply.
-    set p' := (p in SProp_op_order _ (_ p)).
-    move=> /(fun f => f p') Htt.
-    estransitivity; last exact Htt; apply: (unbox (He _ _ _)).
-Qed.
+  (** FIXME: Copy-paste from GenericRulesComplex *)
+  Let valid := valid M01 M02 Wrel θ.
+  Let mk_progSpec := mk_progSpec M01 M02 Wrel.
+
+  Notation " Γ ⊫ c1 ≈ c2 [{ w1 , w2 , w }] " :=
+    (valid Γ _ _ (mk_progSpec Γ _ _ c1 w1 c2 w2 w))
+        (at level 85).
+
+  Ltac destruct_valid :=
+    unshelve econstructor; [split=> /= γ|move=> /= γl γr γw]; constructor.
+  (** FIXME: Copy-paste from GenericRulesComplex *)
+
+  Program Definition raise_spec {Γ} : Γ --> W1 False :=
+    fun=>⦑fun p pexc => pexc tt⦒.
+  Next Obligation. cbv ; intuition. Qed.
+
+  Program Definition rel_raise_spec {Γ A2} (a2: πr Γ -> A2) : ⟬Γ⟭ --> Wrc ⟨False, A2⟩ :=
+    fun γ => ⦑fun p => p ⟨None, a2 (πr γ)⟩⦒.
+  Next Obligation. cbv ; intuition. Qed.
+
+  Lemma ValidRaise Γ A2 (a2: _ -> A2) :
+    Γ ⊫ fun=> raise tt ≈ ret \o a2 [{raise_spec, retW \o a2, rel_raise_spec a2}].
+  Proof. destruct_valid; cbv ; intuition. Qed.
+
+
+  Definition catchStr {Γ E A} (m : Γ -> Exn E A) (merr : Γ × E -> Exn E A)
+    : Γ -> Exn E A := fun γ => catch (m γ) (fun e => merr ⟨γ,e⟩).
+
+  Program Definition catch_spec_str {Γ A1} (w:Γ --> W1 A1)
+          (werr : Γ × unit --> W1 A1) : Γ --> W1 A1 :=
+    fun γ => ⦑fun p pexc => (w γ)∙1 p (fun u => (werr ⟨γ,u⟩)∙1 p pexc)⦒.
+  Next Obligation.
+    cbv ; intuition.
+    move: H1; apply: (w _)∙2=> // ?; apply (werr _)∙2 => //.
+  Qed.
+
+  Program Definition rel_catch_spec_str
+          {Γ A1 A2} (wmrel : ⟬Γ⟭ --> Wrc ⟨A1, A2⟩)
+          (wmerr_rel : ⟬extends Γ unit A2⟭ --> Wrc ⟨A1, A2⟩)
+    : ⟬Γ⟭ --> Wrc ⟨A1, A2⟩ :=
+    fun γ =>
+      ⦑fun p =>
+        let k ae12 :=
+            match nfst ae12 with
+            | Some a1 => p ⟨Some a1, nsnd ae12⟩
+            | None =>
+              (wmerr_rel (extend_point γ tt (nsnd ae12)))∙1 p
+            end
+        in
+        (wmrel γ)∙1 k⦒.
+  Next Obligation.
+    cbv. move=> p1 p2 Hp ; apply: (wmrel _)∙2=> [[[?|] ?]] ; first by apply: Hp.
+    apply: (wmerr_rel _)∙2=> ?; apply: Hp.
+  Qed.
+
+
+  Lemma ValidCatch Γ A1 A2 (m1 : _ -> M1 A1) wm1
+        (m2: _ -> M2 A2) wm2 wmrel merr wmerr wmerr_rel:
+    Γ ⊫ m1 ≈ m2 [{wm1, wm2, wmrel}] ->
+    extends Γ unit A2 ⊫ merr ≈ ret \o nsnd [{wmerr, retW \o nsnd, wmerr_rel}] ->
+    Γ ⊫ catchStr m1 merr ≈ m2
+      [{catch_spec_str wm1 wmerr, wm2, rel_catch_spec_str wmrel wmerr_rel}].
+  Proof.
+    move=> [[/= H1 H2] H] [[/= He1 He2] He]; destruct_valid.
+    - move=> p pexc /=.
+      move: (unbox (H1 γ)); unfold θ01_helper, catchStr.
+      move: (m1 γ) => [?|[[]]?] /=; first apply.
+      set pexc' := (pexc in SProp_op_order _ (_ _ pexc)).
+      move=> /(fun f => f p pexc') Htt.
+      estransitivity; [apply: (unbox (He1 ⟨γ, tt⟩)) | exact Htt].
+    - apply: (unbox (H2 _)).
+    - move=> p /=.
+      move: (unbox (H γl γr γw)); unfold θ01_helper, catchStr.
+      move: (m1 γl) => [?|[[]]?] /=; first apply.
+      set p' := (p in SProp_op_order _ (_ p)).
+      move=> /(fun f => f p') Htt.
+      estransitivity; last exact Htt; apply: (unbox (He _ _ _)).
+  Qed.
+
+End ExcId.
+
+Module ExcExc.
+  Context (E1 E2 : Type).
+
+  Definition M01 := Exn E1.
+  Definition M02 := Exn E2.
+  Definition W01 := ExnSpec E1.
+  Definition W02 := ExnSpec E2.
+
+  Definition M1 := monad_to_relmon M01.
+  Definition M2 := monad_to_relmon M02.
+  Definition W1 := ordmonad_to_relmon W01.
+  Definition W2 := ordmonad_to_relmon W02.
+
+  Import SPropNotations.
+  Import RelNotations.
+
+  Program Definition Wrel0 (A : TypeCatSq) : OrdCat :=
+    dpair _ (MonoContSProp ((nfst A + E1) × (nsnd A + E2))) ⦑@omon_rel _ _⦒.
+  Next Obligation. apply: MonoCont_order_preorder. Qed.
+
+
+  Program Definition retWrel0 (A : TypeCatSq) : OrdCat⦅ Jprod A; Wrel0 A⦆ :=
+    let f : (typeCat_prod A --> Wrel0 A) :=
+        fun a12 => ⦑fun p => p ⟨inl (nfst a12), inl (nsnd a12)⟩⦒
+    in to_discr f.
+  Next Obligation. cbv ; intuition. Qed.
+
+  Program Definition actWrel0 A1 A2 B1 B2 :
+    OrdCat ⦅ discr A1; W1 B1 ⦆ ->
+    OrdCat ⦅ discr A2; W2 B2 ⦆ ->
+    OrdCat ⦅ Jprod ⟨ A1, A2 ⟩; Wrel0 ⟨ B1, B2 ⟩ ⦆ ->
+    OrdCat ⦅ Wrel0 ⟨ A1, A2 ⟩; Wrel0 ⟨ B1, B2 ⟩ ⦆ :=
+    fun wf1 wf2 wfrel =>
+      ⦑fun wm =>
+        ⦑fun p =>
+            let k a12 :=
+                match nfst a12, nsnd a12 with
+                | inl a1, inl a2 => (wfrel∙1 ⟨a1, a2⟩)∙1 p
+                | inr e1, inl a2 => (wf2∙1 a2)∙1 (fun b2 => p ⟨inr e1, inl b2⟩)
+                                             (fun e2 => p ⟨inr e1, inr e2⟩)
+                | inl a1, inr e2 => (wf1∙1 a1)∙1 (fun b1 => p ⟨inl b1, inr e2⟩)
+                                             (fun e1 => p ⟨inr e1, inr e2⟩)
+                | inr e1, inr e2 => p ⟨inr e1, inr e2⟩
+                end
+            in wm∙1 k⦒⦒.
+  Next Obligation.
+    move=> ? ? H; apply: wm∙2 => -[[?|?] [?|?]] //=;
+      set w := (w in w ∙1); by apply: w∙2.
+  Qed.
+  Next Obligation. cbv;intuition. Qed.
+
+  Program Definition Wrc : rsm_components W1 W2 :=
+    mkRSMComponents _ _ Wrel0 retWrel0 actWrel0 _ _ _ _.
+  Next Obligation.
+    move=> ? ? H ? ? H1 ? ? H2 w ? /=.
+    apply: w∙2=> -[[?|?] [?|?]] //= ; [apply: H2 | apply: H | apply: H1].
+  Qed.
+  Next Obligation.
+    apply Ssig_eq=> /=.
+    extensionality wm. apply Ssig_eq. extensionality p=> /=.
+    f_equal. extensionality a; move: a => [[?|?] [?|?]] //=.
+  Qed.
+
+  Definition Wrel : RelationalSpecMonad := mkRSM W1 W2 Wrc.
+
+End ExcExc.
